{
  "nbformat": 4,
  "nbformat_minor": 0,
  "metadata": {
    "colab": {
      "provenance": []
    },
    "kernelspec": {
      "name": "python3",
      "display_name": "Python 3"
    },
    "language_info": {
      "name": "python"
    }
  },
  "cells": [
    {
      "cell_type": "markdown",
      "source": [
        "![image](https://user-images.githubusercontent.com/126839725/228459382-379f8811-72f5-4f49-a95c-4869ab9f0008.png)\n",
        "\n",
        "According to the Euler Beam equation,\n",
        "\n",
        "$${{\\partial^2 y} \\over {\\partial t^2}} +\\frac{EI} {\\rho A}{{\\partial^4 y} \\over {\\partial x^4}}=q(t,x)$$\n",
        "\n",
        "where $y$ is the transverse displacement of the beam, $\\rho$ is the density of the material of the beam, and $E$ is the modulus of rigidity, $I$is the cross sectional moment of inertia, and $A$ is the cross sectional area of the uniform beam.\n",
        "\n",
        "$${{\\partial^2 y} \\over {\\partial t^2}} +\\frac{EI} {\\rho A}{{\\partial^4 y} \\over {\\partial x^4}}=0$$\n",
        "\n",
        "for sovle the 4th order diffrential equation use the method of separation variable method.\n",
        "\n",
        "$$y(x,t) = Y(x)e^{j\\omega t}$$\n",
        "\n",
        "$${{\\partial y(x,t)} \\over {\\partial t}} = j\\omega Y(x) e^{j\\omega t}$$\n",
        "\n",
        "$${{\\partial^2 y(x,t)} \\over {\\partial t^2}} = -\\omega^2Y(x) e^{j\\omega t}$$\n",
        "\n",
        "Substitiut to the homogeneous Euler beam equation,\n",
        "\n",
        "$$e^{j\\omega t}\\frac{EI}{A\\rho}\\frac{d^4 Y(x)}{dx^4}-\\omega^2e^{j\\omega t}Y(x) = 0$$\n",
        "\n",
        "$$\\frac{EI}{A\\rho}\\frac{d^4 Y(x)}{dx^4}-\\omega^2Y(x) = 0$$\n",
        "\n",
        "$$\\frac{d^4 Y(x)}{dx^4}-\\omega^2\\left[\\frac{A\\rho}{EI}\\right]Y(x) = 0$$\n",
        "\n",
        "thake $\\beta$ as,           $\\omega^2\\left[\\frac{A\\rho}{EI}\\right] = \\beta^4$\n",
        "\n",
        "$$\\frac{d^4 Y(x)}{dx^4}-\\beta^4Y(x) = 0$$\n",
        "\n",
        "The spetial solution has the form,\n",
        "\n",
        "$$Y(x) = a_1sinh(\\beta x)+a_2cosh(\\beta x)+a_3sin(\\beta x)+a_4cos(\\beta x)$$\n",
        "\n",
        "$$\\frac{dY(x)}{dx} = a_1\\beta cosh(\\beta x)+a_2\\beta sinh(\\beta x)+a_3\\beta cos(\\beta x)-a_4\\beta sin(\\beta x)$$\n",
        "\n",
        "$$\\frac{d^2Y(x)}{dx^2} = a_1\\beta^2 sinch(\\beta x)+a_2\\beta^2 cosh(\\beta x)-a_3\\beta^2 sin(\\beta x)-a_4\\beta^2 cos(\\beta x)$$\n",
        "\n",
        "$$\\frac{d^3Y(x)}{dx^3} = a_1\\beta^3 cosh(\\beta x)+a_2\\beta^3 sinh(\\beta x)-a_3\\beta^3 cos(\\beta x)+a_4\\beta^3 sin(\\beta x)$$\n",
        "\n",
        "$$\\frac{d^4Y(x)}{dx^4} = a_1\\beta^4 sinh(\\beta x)+a_2\\beta^4 cosh(\\beta x)+a_3\\beta^4 sin(\\beta x)+a_4\\beta^4 cos(\\beta x)$$\n",
        "\n",
        "$$\\frac{d^4Y(x)}{dx^4} = \\beta^4[a_1 sinh(\\beta x)+a_2 cosh(\\beta x)+a_3 sin(\\beta x)+a_4cos(\\beta x)]$$\n",
        "\n",
        "Substitiute the sptial solution into the differential equation,\n",
        "\n",
        "$$\\beta^4[a_1 sinh(\\beta x)+a_2 cosh(\\beta x)+a_3 sin(\\beta x)+a_4cos(\\beta x)]-\\beta^4[a_1 sinh(\\beta x)+a_2 cosh(\\beta x)+a_3 sin(\\beta x)+a_4cos(\\beta x)] = 0$$\n",
        "\n",
        "the equation is satisfied\n",
        "consider the boundary conditions,\n",
        "\\begin{align}\n",
        "y(0) &= 0\\\\\n",
        "Y(0) &= a_1sinh(0)+a_2cosh(0)+a_3sin(0)+a_4cos(0) = 0\\\\\n",
        "a_2+a_4 &= 0\\\\\n",
        "\\frac{dY(0)}{dx} &= 0\\\\\n",
        "\\frac{dY(x)}{dx} &= a_1\\beta cosh(0)+a_2\\beta sinh(0)+a_3\\beta cos(0)-a_4\\beta sin(0)=0\\\\\n",
        "a_1+a_3 &= 0\n",
        "\\end{align}\n",
        "\n",
        "\n",
        "moment(M) and the shear force(V) at the free end are zero,\n",
        "\\begin{align}\n",
        "M &= \\left[EI\\frac{d^2Y(x)}{dX^2}\\right]|_{x=L} = 0\\\\\n",
        "M &= EI\\beta^2[a_1 sinch(\\beta L)+a_2cosh(\\beta L)-a_3 sin(\\beta L)-a_4cos(\\beta L)] = 0\\\\\n",
        "0 &=a_1(sinch(\\beta L)+sin(\\beta L))+a_2(cosh(\\beta L)+cos(\\beta L))\\\\\n",
        "V &= \\frac{d}{dx}\\left[EI\\frac{d^2Y(x)}{dX^2}\\right]|_{x=L} = 0\\\\\n",
        "V &=MI\\beta^3[a_1cosh(\\beta x)+a_2sinh(\\beta x)-a_3cos(\\beta x)+a_4sin(\\beta x)]\\\\\n",
        "0 &=MI\\beta^3[a_1cosh(\\beta L)+a_2sinh(\\beta L)+a_1cos(\\beta L)-a_2sin(\\beta L)]\\\\\n",
        "0 &= a_1(cosh(\\beta xL+cos(\\beta L))+a_2(sinh(\\beta L)-sin(\\beta L))\n",
        "\\end{align}\n",
        "\n",
        "Solve this 2 equation both $a_1$ and $a_2$ are zero\n",
        "\n",
        "there is infinite number of non-dimensional frequencies and eigen valus for each problem. back to the equation, we can rearrange it for the eigen vectors to determine the corresponding eigen function, the equation will become,\n",
        "\n",
        "\\begin{align}\n",
        "y(x,t) &= Y(x)[Acos(\\omega t)+Bsin(\\omega t)]\\\\\n",
        "Y(X) &= a_1sinh(\\beta t)+a_2cos(\\beta t)+a_3sin(\\beta t) +a_4cos(beta t)\\\\\n",
        "Y(x) = \\left[-\\left[\\frac{cosh(\\beta x)-cos(\\beta x)}{sinh(\\beta x)-sin(\\beta x)}\\right][sinh(\\beta x)-sin(\\beta x)+cosh(\\beta x)-cos(\\beta x)]\\right]\n",
        "\\end{align}\n",
        "\n",
        "$Y(x)$ is the characteristic equation for each frequencies.\n",
        "\n",
        "\\begin{align}\n",
        "y(x,t) &= Y_n(x)[A_ncos(\\omega t)+B_nsin(\\omega t)]\\\\\n",
        "y(x,t) &= \\left[-\\left[\\frac{cosh(\\beta_n x)-cos(\\beta_n x)}{sinh(\\beta_n x)-sin(\\beta_n x)}\\right][sinh(\\beta_n x)-sin(\\beta_n x)+cosh(\\beta_n x)-cos(\\beta_n x)]\\right][A_ncos(\\omega_n t)+B_nsin(\\omega_n t)] \n",
        "\\end{align}\n",
        "\n",
        "determine $A_n$ and $B_n$ initial conditions, $y(0,t) = 0$ and ${\\partial y(0,t) \\over \\partial x} = 0$\n",
        "\n",
        "both parameters are constanst and depend on the inertial condiation,\n",
        "\\begin{align}\n",
        "\\begin{bmatrix}y(x,t) = \\phi\\\\{\\partial y(0,t) \\over \\partial x} = \\zeta\\end{bmatrix} where \\  0 <x<L\\\\\n",
        "\\phi(x) &= \\sum_{n=1}^\\infty A_n Y_n(x)dx\\\\\n",
        "\\zeta(x) &= \\sum_{n=1}^\\infty \\omega_n B_n Y_n(x)dx\\\\\n",
        "\\end{align}\n",
        "\n",
        "These equations are analogous to the Fourier series expansions. Thus, both equations are determining the series expansions of\n",
        "the functions $\\phi(x)$, $z\\zeta(x)$ in terms of the characteristic functions $Y(x)$\n",
        "Finally, to find the constants $A_n$ and $B_n$\n",
        "we make use of the orthogonality for the characteristic functions; thus, by\n",
        "integrating these equations with respect to (x) from 0 to L and multiplying by $Y_n(x)$ we get the formulas for $A_n$ and $B_n$\n",
        "\n",
        "\\begin{align}\n",
        "A_n  &= \\frac{2}{L}\\int_{0}^x \\phi(x)Y_n(x)dx\\\\\n",
        "B_n &= \\frac{2}{\\omega_n L}\\int_{0}^{L}\\zeta(x)Y_n(x)dx\n",
        "\\end{align}"
      ],
      "metadata": {
        "id": "5bcpfIEWtG0q"
      }
    }
  ]
}